examples/AsmCombinators.v
@@ -1,0 +1,211 @@
+(** * Composition of [asm] programs *)
+
+Require Import Asm.
+
+From Coq Require Import
+     List
+     Strings.String
+     Program.Basics.
+Import ListNotations.
+From ITree Require Import Basics_Functions.
+Require Import ZArith.
+
+Typeclasses eauto := 5.
+
+(** ** Internal structures *)
+
+Definition fmap_branch {A B : Type} (f: A -> B): branch A -> branch B :=
+  fun b =>
+    match b with
+    | Bjmp a => Bjmp (f a)
+    | Bbrz c a a' => Bbrz c (f a) (f a')
+    | Bhalt => Bhalt
+    end.
+
+Definition fmap_block {A B: Type} (f: A -> B): block A -> block B :=
+  fix fmap b :=
+    match b with
+    | bbb a => bbb (fmap_branch f a)
+    | bbi i b => bbi i (fmap b)
+    end.
+
+Definition relabel_bks {A B C D : Type} (f : A -> B) (g : C -> D)
+           (b : bks B C) : bks A D :=
+  fun a => fmap_block g (b (f a)).
+
+Section after.
+Context {A : Type}.
+Fixpoint after (is : list instr) (bch : branch A) : block A :=
+  match is with
+  | nil => bbb bch
+  | i :: is => bbi i (after is bch)
+  end.
+End after.
+
+(** ** Low-level interface with [asm] *)
+
+(** Any collection of blocks forms an [asm] program with
+      no hidden blocks. *)
+Definition raw_asm {A B} (b : bks A B) : asm A B :=
+  {| internal := Empty_set;
+     code := fun a' =>
+               match a' with
+               | inl v => match v : Empty_set with end
+               | inr a => fmap_block inr (b a)
+               end;
+  |}.
+
+(** Wrap a single block as [asm]. *)
+Definition raw_asm_block {A} (b : block A) : asm unit A :=
+  raw_asm (fun _ => b).
+
+(** ** [asm] combinators *)
+
+(** An [asm] program made only of external jumps. This is
+      useful to connect programs with [app_asm]. *)
+Definition pure_asm {A B} (f : A -> B) : asm A B :=
+  raw_asm (fun a => bbb (Bjmp (f a))).
+
+Definition id_asm {A} : asm A A := pure_asm id.
+
+(* Internal relabeling functions for [app_asm] *)
+Definition _app_B {I J B D} :
+  block (I + B) -> block ((I + J) + (B + D)) :=
+  fmap_block (fun l =>
+                match l with
+                | inl i => inl (inl i)
+                | inr b => inr (inl b)
+                end).
+
+Definition _app_D {I J B D} :
+  block (J + D) -> block ((I + J) + (B + D)) :=
+  fmap_block (fun l =>
+                match l with
+                | inl j => inl (inr j)
+                | inr d => inr (inr d)
+                end).
+
+(** Append two asm programs, preserving their internal links. *)
+Definition app_asm {A B C D} (ab : asm A B) (cd : asm C D) :
+  asm (A + C) (B + D) :=
+  {| internal := ab.(internal) + cd.(internal);
+     code := fun l =>
+               match l with
+               | inl (inl ia) => _app_B (ab.(code) (inl ia))
+               | inl (inr ic) => _app_D (cd.(code) (inl ic))
+               | inr (inl  a) => _app_B (ab.(code) (inr  a))
+               | inr (inr  c) => _app_D (cd.(code) (inr  c))
+               end;
+  |}.
+
+(** Rename visible program labels. *)
+Definition relabel_asm {A B C D} (f : A -> B) (g : C -> D)
+           (bc : asm B C) : asm A D :=
+  {| code := relabel_bks (sum_bimap id f) (sum_bimap id g) bc.(code);
+  |}.
+
+(** Link labels from two programs together. *)
+Definition link_asm {I A B} (ab : asm (I + A) (I + B)) : asm A B :=
+  {| internal := ab.(internal) + I;
+     code := relabel_bks sum_assoc_r sum_assoc_l ab.(code);
+  |}.
+
+(** ** Correctness *)
+(** The combinators above map to their denotational counterparts. *)
+
+From ExtLib Require Import
+     Structures.Monad.
+Import MonadNotation.
+From ITree Require Import
+     ITree OpenSum Fix.
+Require Import Imp Den.
+
+Section Correctness.
+
+Context {E : Type -> Type}.
+Context {HasLocals : Locals -< E}.
+Context {HasMemory : Memory -< E}.
+
+(** *** Internal structures *)
+
+Lemma fmap_block_map:
+  forall  {L L'} b (f: L -> L'),
+    denote_block E (fmap_block f b) ≅ ITree.map (sum_bimap f id) (denote_block E b).
+Proof.
+  induction b as [i b | br]; intros f.
+  - simpl.
+    unfold ITree.map; rewrite bind_bind.
+    eapply eq_itree_eq_bind; [reflexivity | intros []; apply IHb].
+  - simpl.
+    destruct br; simpl.
+    + unfold ITree.map; rewrite ret_bind; reflexivity.
+    + unfold ITree.map; rewrite bind_bind.
+      eapply eq_itree_eq_bind; [reflexivity | intros []; rewrite ret_bind; reflexivity].
+    + unfold ITree.map; rewrite ret_bind; reflexivity.
+Qed.
+
+Definition traverse_ {A: Type} {M: Type -> Type} `{Monad M} (f: A -> M unit): list A -> M unit :=
+  fix traverse__ l: M unit :=
+    match l with
+    | [] => ret tt
+    | a::l => (f a;; traverse__ l)%monad
+    end.
+
+Definition denote_list: list instr -> itree E unit :=
+  traverse_ (denote_instr E).
+
+Lemma denote_after_denote_list:
+  forall {label: Type} instrs (b: branch label),
+    denote_block E (after instrs b) ≅ (denote_list instrs ;; denote_branch E b).
+Proof.
+  induction instrs as [| i instrs IH]; intros b.
+  - simpl; rewrite ret_bind; reflexivity.
+  - simpl; rewrite bind_bind.
+    eapply eq_itree_eq_bind; [reflexivity | intros []; apply IH].
+Qed.
+
+Lemma denote_list_app:
+  forall is1 is2,
+    @denote_list (is1 ++ is2) ≅
+                 (@denote_list is1;; denote_list is2).
+Proof.
+  intros is1 is2; induction is1 as [| i is1 IH]; simpl; intros; [rewrite ret_bind; reflexivity |].
+  rewrite bind_bind; setoid_rewrite IH; reflexivity.
+Qed.
+
+(** *** [asm] combinators *)
+
+Theorem pure_asm_correct {A B} (f : A -> B) :
+  eq_den (denote_asm (pure_asm f))
+         (@lift_den E _ _ f).
+Proof.
+Admitted.
+
+Definition id_asm_correct {A} :
+  eq_den (denote_asm (pure_asm id)) (@id_den E A).
+Proof.
+Admitted.
+
+Definition app_asm_correct {A B C D} (ab : asm A B) (cd : asm C D) :
+  @eq_den E _ _
+     (denote_asm (app_asm ab cd))
+     (tensor_den (denote_asm ab) (denote_asm cd)).
+Proof.
+Admitted.
+
+Definition relabel_asm_correct {A B C D} (f : A -> B) (g : C -> D)
+           (bc : asm B C) :
+  @eq_den E _ _
+     (denote_asm (relabel_asm f g bc))
+     (lift_den f >=> denote_asm bc >=> lift_den g).
+Proof.
+Admitted.
+
+Definition link_asm_correct {I A B} (ab : asm (I + A) (I + B)) :
+  @eq_den E _ _
+     (denote_asm (link_asm ab))
+     (loop_den (denote_asm ab)).
+Proof.
+Admitted.
+
+End Correctness.
